crypto_examples/mulntt_ct/mulntt_ct_rec.dfy
@@ -1,234 +1,18 @@
-include "twiddle_factors.dfy"
+include "nth_root.dfy"
 
-module mulntt_ct_rec {
+abstract module mulntt_ct_rec {
     import opened Seq
     import opened Power
     import opened Power2
     import opened DivMod
     import opened Mul
 
-    import opened pows_of_2
-
-    import opened nth_root
+	import opened pows_of_2
     import opened ntt_index
+    import opened nth_root
     import opened ntt_polys
-    import opened twiddle_factors
 
-    predicate {:opaque} unifromly_sized(blocks: seq<seq<elem>>, bsize: pow2_t)
-        requires bsize.exp <= LOGN;
-        ensures unifromly_sized(blocks, bsize)
-            ==> |blocks| == block_count(bsize).full;
-    {
-        && (forall i: nat | i < |blocks| :: |blocks[i]| == bsize.full)
-        && |blocks| == block_count(bsize).full
-    }
-
-    lemma unifromly_sized_instance_lemma(blocks: seq<seq<elem>>, bsize: pow2_t, i: nat)
-        requires bsize.exp <= LOGN;
-        requires unifromly_sized(blocks, bsize);
-        requires i < |blocks|;
-        ensures |blocks[i]| == bsize.full;
-    {
-        reveal unifromly_sized();
-    }
-
-    lemma point_view_index_bound_lemma(i: nat, j: nat, bsize: pow2_t)
-        requires bsize.exp <= LOGN;
-        requires i < block_count(bsize).full;
-        requires j < bsize.full;
-        ensures 0 <= i + j * block_count(bsize).full < N;
-    {
-        var count := block_count(bsize).full;
-        calc {
-            i + j * count;
-            <=
-            count - 1 + j * count;
-            <= { LemmaMulInequality(j, bsize.full - 1, count); }
-            count - 1 + (bsize.full - 1) * count;
-            { LemmaMulIsDistributive(count, bsize.full, 1); }
-            count - 1 + bsize.full * count - count;
-            bsize.full * count - 1;
-            { Nth_root_lemma(); }
-            N - 1;
-        }
-
-        LemmaMulStrictlyPositiveAuto();
-    }
-
-    function point_view_index(i: nat, j: nat, bsize: pow2_t): (offset: nat)
-        requires bsize.exp <= LOGN;
-        requires i < block_count(bsize).full;
-        requires j < bsize.full;
-        ensures offset < N;
-    {
-        point_view_index_bound_lemma(i, j, bsize);
-        i + j * block_count(bsize).full
-    }
-
-    lemma point_view_index_disjont_lemma(i: nat, j: nat, i': nat, j': nat, bsize: pow2_t)
-        requires bsize.exp <= LOGN;
-        requires i < block_count(bsize).full;
-        requires j < bsize.full;
-        requires i' < block_count(bsize).full;
-        requires j' < bsize.full;
-        requires i != i' || j != j';
-        ensures point_view_index(i, j, bsize) != point_view_index(i', j', bsize);
-    {
-        var offset := point_view_index(i, j, bsize);
-        var offset' := point_view_index(i', j', bsize);
-        var count := block_count(bsize).full;
-
-        if i != i' && offset == offset' {
-            LemmaFundamentalDivModConverse(offset, count, j, i);
-            LemmaFundamentalDivModConverse(offset, count, j', i');
-            assert false;
-            return;
-        }
-
-        if j != j' && offset == offset' {
-            assert i == i';
-            assert j * count == j' * count;
-            LemmaMulIsCommutativeAuto();
-            LemmaMulEqualityConverse(count, j', j);
-            assert false;
-        }
-    }
-
-    function points_view(a: n_sized, i: nat, bsize: pow2_t): (v: seq<elem>)
-        requires bsize.exp <= LOGN;
-        requires i < block_count(bsize).full;
-        // ensures |v| == bsize.full;
-    {
-        var size := bsize.full;
-        seq(size, j requires 0 <= j < size => a[point_view_index(i, j, bsize)])
-    }
-
-    // interpret an n_sized buffer as a level view
-    // contains blocks of points, each block has bsize
-    function level_points_view(a: n_sized, bsize: pow2_t): (vs: seq<seq<elem>>)
-        requires bsize.exp <= LOGN;
-        ensures unifromly_sized(vs, bsize);
-    {
-        var count := block_count(bsize).full;
-        var vs := seq(count, i requires 0 <= i < count => points_view(a, i, bsize));
-        assert unifromly_sized(vs, bsize) by {
-            reveal unifromly_sized();
-        }
-        vs
-    }
-
-    function method {:opaque} build_lower_level(higher: seq<seq<elem>>, bsize: pow2_t): (lower: seq<seq<elem>>)
-        requires 1 <= bsize.exp <= LOGN;
-        requires unifromly_sized(higher, bsize);
-        ensures unifromly_sized(lower, pow2_half(bsize));
-    {
-        reveal unifromly_sized();
-        pow2_basics(bsize);
-        block_count_half_lemma(bsize);
-        var new_size := pow2_half(bsize);
-        var new_count := |higher| * 2;
-        seq(new_count, n requires 0 <= n < new_count => 
-            if n % 2 == 0 then even_indexed_items(higher[n/2], bsize)
-            else odd_indexed_items(higher[n/2], bsize))
-    }
-
-    function method {:opaque} build_higher_level(lower: seq<seq<elem>>, bsize: pow2_t): (higher: seq<seq<elem>>)
-        requires 0 <= bsize.exp < LOGN;
-        requires unifromly_sized(lower, bsize);
-        ensures unifromly_sized(higher, pow2_double(bsize));
-    {
-        reveal unifromly_sized();
-        pow2_basics(bsize);
-        var new_size := pow2_double(bsize);
-        block_count_half_lemma(new_size);
-        var new_count := |lower| / 2;
-        seq(new_count, n requires 0 <= n < new_count => 
-            merge_even_odd_indexed_items(lower[n*2], lower[n*2+1], bsize))
-    }
-
-    lemma build_higher_inverse_lemma(lower: seq<seq<elem>>, bsize: pow2_t)
-        requires 0 <= bsize.exp < LOGN;
-        requires unifromly_sized(lower, bsize);
-        ensures build_lower_level(build_higher_level(lower, bsize), pow2_double(bsize)) == lower;
-    {
-        reveal build_higher_level();
-        reveal build_lower_level();
-        var higher := build_higher_level(lower, bsize);
-        var new_size := pow2_double(bsize);
-        assert build_lower_level(higher, new_size) == lower;
-    }
-
-    lemma poly_base_level_correct_lemma()
-        ensures unifromly_sized([A()], pow2(LOGN));
-    {
-        reveal unifromly_sized();
-    }
-
-    // construct polys level view 
-    // each block is a poly, has bsize coefficients
-    function level_polys(bsize: pow2_t): (lps: seq<seq<elem>>)
-        requires 0 <= bsize.exp <= LOGN;
-        decreases LOGN - bsize.exp;
-        ensures unifromly_sized(lps, bsize);
-    {
-        if bsize.exp == LOGN then
-            poly_base_level_correct_lemma();
-            [A()]
-        else
-            var double_size := pow2_double(bsize);
-            var higher := level_polys(double_size);
-            build_lower_level(higher, double_size)
-    }
-
-    lemma level_polys_index_correspondence_lemma(
-        higher: seq<seq<elem>>, hi_size: pow2_t, i: nat, 
-        lower: seq<seq<elem>>)
-        requires 1 <= hi_size.exp <= LOGN;
-        requires i < |higher|;
-        requires unifromly_sized(higher, hi_size);
-        requires build_lower_level(higher, hi_size) == lower;
-        ensures |higher[i]| == hi_size.full;
-        ensures 2 * i + 1 < |lower|;
-        ensures even_indexed_items(higher[i], hi_size) == lower[2 * i];
-        ensures odd_indexed_items(higher[i], hi_size) == lower[2 * i + 1];
-        ensures |lower[2 * i]| == |lower[2 * i + 1]| == pow2_half(hi_size).full;
-    {
-        reveal unifromly_sized();
-        reveal build_lower_level();
-    }
-
-    predicate {:opaque} points_eval_prefix_inv(points: seq<elem>, poly: seq<elem>, l: nat, count: pow2_t)
-    {
-        && count.exp <= LOGN
-        && l <= |points| == |poly| == block_size(count).full
-        && (forall i | 0 <= i < l :: poly_eval(poly, x_value(i, count)) == points[i])
-    }
-
-    lemma points_eval_prefix_inv_vacuous_lemma(points: seq<elem>, poly: seq<elem>, count: pow2_t)
-        requires count.exp <= LOGN;
-        requires |points| == |poly| == block_size(count).full;
-        ensures points_eval_prefix_inv(points, poly, 0, count);
-    {
-        forall i | 0 <= i < 0 
-            ensures poly_eval(poly, x_value(i, count)) == points[i];
-        {
-        }
-        reveal points_eval_prefix_inv();
-    }
-
-    // d is the block count
-    predicate {:opaque} points_eval_suffix_inv(points: seq<elem>, poly: seq<elem>, l: nat, count: pow2_t)
-    {
-        && count.exp <= LOGN
-        && l <= |points| == |poly| == block_size(count).full
-        && (forall i | l <= i < block_size(count).full ::
-            poly_eval(poly, x_value(i, count)) == points[i])
-    }
-
-    predicate points_eval_inv(points: seq<elem>, poly: seq<elem>, count: pow2_t)
-    {
-        points_eval_suffix_inv(points, poly, 0, count)
-    }
+    const x_value: x_fun := rev_mixed_powers_mont_x_value;
 
     datatype loop_view = loop_view(
         lower: seq<seq<elem>>, // lower polys
@@ -237,7 +21,7 @@ module mulntt_ct_rec {
     {
         predicate loop_view_wf()
         {
-            && 1 <= hsize.exp <= LOGN
+            && 1 <= hsize.exp <= N.exp
             && unifromly_sized(higher, hsize)
             && build_lower_level(higher, hsize) == lower
         }
@@ -265,40 +49,40 @@ module mulntt_ct_rec {
             ensures pow2_double(lsize()) == hsize;
             ensures lcount() == pow2_double(hcount());
             ensures lcount().full * lsize().full
-                == hcount().full * hsize.full == N;
+                == hcount().full * hsize.full == N.full;
         {
             Nth_root_lemma();
             block_count_half_lemma(hsize);
         }
 
         predicate {:opaque} t_loop_low_inv(a: n_sized, hcount: pow2_t)
-            requires hcount.exp < LOGN;
+            requires hcount.exp < N.exp;
             requires loop_view_wf();
             requires hsize == block_size(hcount);
         {
             && var lcount := lcount();
             && var lpoints := level_points_view(a, lsize());
             && (forall i | 0 <= i < lcount.full ::
-                points_eval_inv(lpoints[i], lower[bit_rev_int(i, lcount)], lcount))
+                points_eval_inv(lpoints[i], lower[bit_rev_int(i, lcount)], rev_mixed_powers_mont_x_value, lcount))
         }
 
         predicate t_loop_inv(a: n_sized, hcount: pow2_t)
         {
             && loop_view_wf()
-            && 0 <= hcount.exp < LOGN
+            && 0 <= hcount.exp < N.exp
             && hsize == block_size(hcount)
             && t_loop_low_inv(a, hcount)
         }
 
-        static function init_loop_view(): (v: loop_view) 
-            ensures v.loop_view_wf();
-        {   
-            var hsize := pow2(1);
-            loop_view(
-                level_polys(pow2_half(hsize)), 
-                level_polys(hsize),
-                hsize)
-        }
+        // static function init_loop_view(): (v: loop_view) 
+        //     ensures v.loop_view_wf();
+        // {   
+        //     var hsize := pow2(1);
+        //     loop_view(
+        //         level_polys(pow2_half(hsize)), 
+        //         level_polys(hsize),
+        //         hsize)
+        // }
 
         // lemma init_loop_view_lemma(a: n_sized)
         //     requires this == init_loop_view();
@@ -311,8 +95,8 @@ module mulntt_ct_rec {
         //     var hcount := hcount();
 
         //     Nth_root_lemma();
-        //     assert lcount == pow2(LOGN); 
-        //     assert hcount == pow2(LOGN-1);
+        //     assert lcount == pow2(N.exp); 
+        //     assert hcount == pow2(N.exp-1);
 
         //     assert t_loop_low_inv(a, hcount) by {
         //         forall i | 0 <= i < lcount.full
@@ -327,18 +111,18 @@ module mulntt_ct_rec {
         predicate t_loop_end(a: n_sized)
         {
             && loop_view_wf()
-            && hsize.exp == LOGN
+            && hsize.exp == N.exp
             && var hpoints := level_points_view(a, hsize);
             && |hpoints| == 1
             && |higher| == 1
-            && points_eval_inv(hpoints[0], higher[0], pow2(0))
+            && points_eval_inv(hpoints[0], higher[0], rev_mixed_powers_mont_x_value, pow2(0))
         }
 
         lemma x_value_even_square_lemma(j: nat, x: elem)
             requires loop_view_wf();
             requires 2 * j < hsize.full;
-            requires x == x_value(2 * j, hcount());
-            ensures modmul(x, x) == x_value(j, lcount());
+            requires x == rev_mixed_powers_mont_x_value(2 * j, hcount());
+            ensures mqmul(x, x) == rev_mixed_powers_mont_x_value(j, lcount());
         {
             size_count_lemma();
             var hc := hcount();
@@ -377,7 +161,7 @@ module mulntt_ct_rec {
             var temp := Pow(PSI, exp);
     
             calc == {
-                modmul(x, x);
+                mqmul(x, x);
                 ((temp % Q) * (temp % Q)) % Q;
                 {
                     LemmaMulModNoopGeneral(temp, temp, Q);
@@ -387,15 +171,15 @@ module mulntt_ct_rec {
                     LemmaPowAdds(PSI, exp, exp);
                 }
                 Pow(PSI, 2 * exp) % Q;
-                x_value(j, lcount());
+                rev_mixed_powers_mont_x_value(j, lcount());
             }
         }
 
         lemma x_value_odd_square_lemma(j: nat, x: elem)
             requires loop_view_wf();
             requires 2 * j < hsize.full;
-            requires x == x_value(2 * j + 1, hcount());
-            ensures modmul(x, x) == x_value(j, lcount());
+            requires x == rev_mixed_powers_mont_x_value(2 * j + 1, hcount());
+            ensures mqmul(x, x) == rev_mixed_powers_mont_x_value(j, lcount());
         {
             size_count_lemma();
             var hc := hcount();
@@ -440,21 +224,23 @@ module mulntt_ct_rec {
                 }
                 2 * (bit_rev_int(j, lsize()) * lcount().full + lsize().full * lcount().full) + lcount().full;
                 {
-                    assert lsize().full * lcount().full == N;
+                    size_count_lemma();
+                    LemmaMulIsCommutative(lsize().full, lcount().full);
+                    assert lsize().full * lcount().full == N.full;
                 }
-                2 * (bit_rev_int(j, lsize()) * lcount().full + N) + lcount().full;
+                2 * (bit_rev_int(j, lsize()) * lcount().full + N.full) + lcount().full;
                 {
-                    LemmaMulIsDistributive(2, bit_rev_int(j, lsize()) * lcount().full, N);
+                    LemmaMulIsDistributive(2, bit_rev_int(j, lsize()) * lcount().full, N.full);
                 }
-                2 * (bit_rev_int(j, lsize()) * lcount().full) + 2 * N + lcount().full;
+                2 * (bit_rev_int(j, lsize()) * lcount().full) + 2 * N.full + lcount().full;
                 {
                     LemmaMulIsAssociativeAuto();
                 }
-                2 * bit_rev_int(j, lsize()) * lcount().full + 2 * N + lcount().full;
+                2 * bit_rev_int(j, lsize()) * lcount().full + 2 * N.full + lcount().full;
             }
 
             calc == {
-                modmul(x, x);
+                mqmul(x, x);
                 ((temp % Q) * (temp % Q)) % Q;
                 {
                     LemmaMulModNoopGeneral(temp, temp, Q);
@@ -464,7 +250,7 @@ module mulntt_ct_rec {
                     LemmaPowAdds(PSI, exp, exp);
                 }
                 Pow(PSI, 2 * exp) % Q;
-                Pow(PSI, 2 * bit_rev_int(j, lsize()) * lcount().full + 2 * N + lcount().full) % Q;
+                Pow(PSI, 2 * bit_rev_int(j, lsize()) * lcount().full + 2 * N.full + lcount().full) % Q;
                 {
                     LemmaMulNonnegative(2 * bit_rev_int(j, lsize()), lcount().full);
                     full_rotation_lemma(2 * bit_rev_int(j, lsize()) * lcount().full + lcount().full);
@@ -474,30 +260,30 @@ module mulntt_ct_rec {
         }
 
         predicate {:opaque} j_loop_higher_inv(a: n_sized, hcount: pow2_t, j: nat)
-            requires hcount.exp <= LOGN;
+            requires hcount.exp <= N.exp;
             requires loop_view_wf();
             requires hsize == block_size(hcount);
         {
             && var hpoints := level_points_view(a, hsize);
             && (forall i | 0 <= i < hcount.full ::
-                points_eval_prefix_inv(hpoints[i], higher[bit_rev_int(i, hcount)], 2*j, hcount))
+                points_eval_prefix_inv(hpoints[i], higher[bit_rev_int(i, hcount)], rev_mixed_powers_mont_x_value, 2*j, hcount))
         }
 
         predicate {:opaque} j_loop_lower_inv(a: n_sized, hcount: pow2_t, j: nat)
-            requires hcount.exp <= LOGN;
+            requires hcount.exp <= N.exp;
             requires loop_view_wf();
             requires hsize == block_size(hcount);
         {
             && var lcount := lcount();
             && var lpoints := level_points_view(a, lsize());
             && (forall i | 0 <= i < lcount.full ::
-                points_eval_suffix_inv(lpoints[i], lower[bit_rev_int(i, lcount)], j, lcount))
+                points_eval_suffix_inv(lpoints[i], lower[bit_rev_int(i, lcount)], rev_mixed_powers_mont_x_value, j, lcount))
         }
 
         predicate j_loop_inv(a: n_sized, hcount: pow2_t, j: nat)
         {
             && loop_view_wf()
-            && hcount.exp <= LOGN
+            && hcount.exp <= N.exp
             && hsize == block_size(hcount)
             && j <= lsize().full
             && j_loop_higher_inv(a, hcount, j)
@@ -505,20 +291,20 @@ module mulntt_ct_rec {
         }
 
         predicate {:opaque} s_loop_higher_inv(a: n_sized, hcount: pow2_t, j: nat, bi: nat)
-            requires hcount.exp <= LOGN;
+            requires hcount.exp <= N.exp;
             requires bi <= hcount.full;
             requires loop_view_wf();
             requires hsize == block_size(hcount);
         {
             && var hpoints := level_points_view(a, hsize);
             && (forall i | 0 <= i < bi ::
-                points_eval_prefix_inv(hpoints[i], higher[bit_rev_int(i, hcount)], 2*j+2, hcount))
+                points_eval_prefix_inv(hpoints[i], higher[bit_rev_int(i, hcount)], rev_mixed_powers_mont_x_value, 2*j+2, hcount))
             && (forall i | bi <= i < hcount.full ::
-                points_eval_prefix_inv(hpoints[i], higher[bit_rev_int(i, hcount)], 2*j, hcount))
+                points_eval_prefix_inv(hpoints[i], higher[bit_rev_int(i, hcount)], rev_mixed_powers_mont_x_value, 2*j, hcount))
         }
 
         predicate {:opaque} s_loop_lower_inv(a: n_sized, hcount: pow2_t, j: nat, bi: nat)
-            requires hcount.exp <= LOGN;
+            requires hcount.exp <= N.exp;
             requires bi <= hcount.full;
             requires loop_view_wf();
             requires hsize == block_size(hcount);
@@ -527,15 +313,15 @@ module mulntt_ct_rec {
             && var lcount := lcount();
             && var lpoints := level_points_view(a, lsize());
             && (forall i | (0 <= i < bi || hcount.full <= i < bi + hcount.full) ::
-                && (points_eval_suffix_inv(lpoints[i], lower[bit_rev_int(i, lcount)], j+1, lcount)))
+                && (points_eval_suffix_inv(lpoints[i], lower[bit_rev_int(i, lcount)], rev_mixed_powers_mont_x_value, j+1, lcount)))
             && (forall i | (bi <= i < hcount.full || bi + hcount.full <= i < lcount.full) ::
-                points_eval_suffix_inv(lpoints[i], lower[bit_rev_int(i, lcount)], j, lcount))
+                points_eval_suffix_inv(lpoints[i], lower[bit_rev_int(i, lcount)], rev_mixed_powers_mont_x_value, j, lcount))
         }
 
         predicate s_loop_inv(a: n_sized, hcount: pow2_t, j: nat, bi: nat)
         {
             && loop_view_wf()
-            && hcount.exp <= LOGN
+            && hcount.exp <= N.exp
             && bi <= hcount.full
             && j < lsize().full
             && hsize == block_size(hcount)
@@ -545,11 +331,11 @@ module mulntt_ct_rec {
 
         // lemma s_loop_index_bound(a: n_sized, hcount: pow2_t, j: nat, bi: nat)
         //     requires loop_view_wf();
-        //     requires hcount.exp <= LOGN;
+        //     requires hcount.exp <= N.exp;
         //     requires bi < hcount.full;
         //     requires j < lsize().full;
         //     requires hsize == block_size(hcount);
-        //     ensures bi + (2*j) * hcount.full + hcount.full < N;
+        //     ensures bi + (2*j) * hcount.full + hcount.full < N.full;
         //     ensures bi + hcount.full < lcount().full;
         // {
         //     size_count_lemma();
@@ -564,7 +350,7 @@ module mulntt_ct_rec {
             requires s_loop_inv(a, hcount, j, bi);
             requires bi < hcount.full
             ensures s == bi + (2*j) * hcount.full;
-            ensures s + hcount.full < N;
+            ensures s + hcount.full < N.full;
             ensures a[s] == level_points_view(a, hsize)[bi][2*j];
             ensures s == point_view_index(bi, 2*j, hsize);
             ensures a[s+hcount.full] == level_points_view(a, hsize)[bi][2*j+1];
@@ -610,7 +396,7 @@ module mulntt_ct_rec {
             requires s_loop_inv(a, hcount, j, bi);
             requires bi < hcount.full
             ensures s == bi + (2*j) * hcount.full;
-            ensures s + hcount.full < N;
+            ensures s + hcount.full < N.full;
             ensures bi + hcount.full < lcount().full;
             ensures a[s] == level_points_view(a, lsize())[bi][j];
             ensures s == point_view_index(bi, j, lsize());
@@ -683,7 +469,7 @@ module mulntt_ct_rec {
             requires s_loop_inv(a, hcount, j, bi);
             requires bi < hcount.full
             requires s == bi + (2*j) * hcount.full;
-            ensures s + hcount.full < N;
+            ensures s + hcount.full < N.full;
             ensures bi + hcount.full < lcount().full;
             ensures a[s] == poly_eval(get_even_poly(bi), x_value(j, lcount()));
             ensures a[s+hcount.full] == poly_eval(get_odd_poly(bi), x_value(j, lcount()));
@@ -697,7 +483,7 @@ module mulntt_ct_rec {
             var e_points := lpoints[bi];
 
             assert a[s] == poly_eval(e_poly, x_value(j, lcount)) by {
-                assert points_eval_suffix_inv(e_points, e_poly, j, lcount) by {
+                assert points_eval_suffix_inv(e_points, e_poly, x_value, j, lcount) by {
                     reveal s_loop_lower_inv();
                 }
                 reveal points_eval_suffix_inv();
@@ -708,7 +494,7 @@ module mulntt_ct_rec {
             var o_points := lpoints[bi+hcount.full];
 
             assert a[s+hcount.full] == poly_eval(o_poly, x_value(j, lcount)) by {
-                assert points_eval_suffix_inv(o_points, o_poly, j, lcount) by {
+                assert points_eval_suffix_inv(o_points, o_poly, x_value, j, lcount) by {
                     reveal s_loop_lower_inv();
                 }
                 reveal points_eval_suffix_inv();
@@ -744,10 +530,10 @@ module mulntt_ct_rec {
             requires s_loop_inv(a, hcount, j, bi);
             requires s == bi + (2*j) * hcount.full;
             requires bi < hcount.full
-            requires w == modmul(x_value(2 * j, hcount), R);
-            ensures s + hcount.full < N;
+            requires w == mqmul(x_value(2 * j, hcount), R);
+            ensures s + hcount.full < N.full;
             ensures bi + hcount.full < lcount().full;
-            ensures poly_eval(get_full_poly(bi), x_value(2*j, hcount)) == modadd(a[s], montmul(a[s+hcount.full], w));
+            ensures poly_eval(get_full_poly(bi), x_value(2*j, hcount)) == mqadd(a[s], montmul(a[s+hcount.full], w));
         {
             size_count_lemma();
             lower_points_view_value_lemma(a, hcount, j, bi, s);
@@ -760,7 +546,7 @@ module mulntt_ct_rec {
                     LemmaSmallMod(p, Q);
                 }
                 assert IsModEquivalent(R_INV * R, 1, Q) by {
-                    R_INV_lemma();
+                    Nth_root_lemma();
                 }
                 assert IsModEquivalent(w, x_value(2 * j, hcount) * R, Q) by {
                     LemmaSmallMod(w, Q);
@@ -771,8 +557,8 @@ module mulntt_ct_rec {
                 LemmaSmallMod(p, Q);
             }
 
-            var sum := modadd(e, p);
-            var diff := modsub(e, p);
+            var sum := mqadd(e, p);
+            var diff := mqsub(e, p);
 
             var e_poly := get_even_poly(bi);
             var o_poly := get_odd_poly(bi);
@@ -795,11 +581,11 @@ module mulntt_ct_rec {
             requires s_loop_inv(a, hcount, j, bi);
             requires bi < hcount.full
             requires s == bi + (2*j) * hcount.full;
-            requires w == modmul(x_value(2 * j, hcount), R);
-            ensures s + hcount.full < N;
+            requires w == mqmul(x_value(2 * j, hcount), R);
+            ensures s + hcount.full < N.full;
             ensures bi + hcount.full < lcount().full;
             ensures poly_eval(get_full_poly(bi), x_value(2*j+1, hcount))
-                == modsub(a[s], montmul(a[s+hcount.full], w));
+                == mqsub(a[s], montmul(a[s+hcount.full], w));
         {
             size_count_lemma();
             lower_points_view_value_lemma(a, hcount, j, bi, s);
@@ -812,7 +598,7 @@ module mulntt_ct_rec {
                     LemmaSmallMod(p, Q);
                 }
                 assert IsModEquivalent(R_INV * R, 1, Q) by {
-                    R_INV_lemma();
+                    Nth_root_lemma();
                 }
                 assert IsModEquivalent(w, x_value(2*j, hcount) * R, Q) by {
                     LemmaSmallMod(w, Q);
@@ -823,7 +609,7 @@ module mulntt_ct_rec {
                 LemmaSmallMod(p, Q);
             }
 
-            var diff := modsub(e, p);
+            var diff := mqsub(e, p);
 
             var e_poly := get_even_poly(bi);
             var o_poly := get_odd_poly(bi);
@@ -843,31 +629,31 @@ module mulntt_ct_rec {
                 {
                     LemmaMulNonnegative(2 * bit_rev_int(2*j+1, hsize), hcount.full);
                 }
-                modpow(PSI, 2 * bit_rev_int(2*j+1, hsize) * hcount.full + hcount.full);
+                mqpow(PSI, 2 * bit_rev_int(2*j+1, hsize) * hcount.full + hcount.full);
                 {
                     bit_rev_int_lemma3(j, lsize());
                     assert bit_rev_int(2*j+1, hsize) == bit_rev_int(j, lsize()) + lsize().full;
                 }
-                modpow(PSI, 2 * (bit_rev_int(j, lsize()) + lsize().full) * hcount.full + hcount.full);
+                mqpow(PSI, 2 * (bit_rev_int(j, lsize()) + lsize().full) * hcount.full + hcount.full);
                 {
-                    gbassert 2 * (bit_rev_int(j, lsize()) + lsize().full) * hcount.full == 2 * (bit_rev_int(j, lsize()) * hcount.full) + N by {
-                        assert 2 * lsize().full * hcount.full == N;
+                    gbassert 2 * (bit_rev_int(j, lsize()) + lsize().full) * hcount.full == 2 * (bit_rev_int(j, lsize()) * hcount.full) + N.full by {
+                        assert 2 * lsize().full * hcount.full == N.full;
                     }
                 }
-                modpow(PSI, 2 * (bit_rev_int(j, lsize()) * hcount.full) + N + hcount.full);
+                mqpow(PSI, 2 * (bit_rev_int(j, lsize()) * hcount.full) + N.full + hcount.full);
                 {
                     LemmaMulNonnegative(bit_rev_int(j, lsize()), hcount.full);
                     half_rotation_lemma(2 * (bit_rev_int(j, lsize()) * hcount.full) + hcount.full);
                 }
-                (Q - modpow(PSI, 2 * (bit_rev_int(j, lsize()) * hcount.full) + hcount.full)) % Q;
+                (Q - mqpow(PSI, 2 * (bit_rev_int(j, lsize()) * hcount.full) + hcount.full)) % Q;
                 {
                     LemmaMulIsAssociative(2, bit_rev_int(j, lsize()), hcount.full);
                 }
-                (Q - modpow(PSI, 2 * bit_rev_int(j, lsize()) * hcount.full + hcount.full)) % Q;
+                (Q - mqpow(PSI, 2 * bit_rev_int(j, lsize()) * hcount.full + hcount.full)) % Q;
                 {
                     bit_rev_int_lemma2(j, lsize());
                 }
-                (Q - modpow(PSI, 2 * bit_rev_int(2*j, hsize) * hcount.full + hcount.full)) % Q;
+                (Q - mqpow(PSI, 2 * bit_rev_int(2*j, hsize) * hcount.full + hcount.full)) % Q;
                 (Q - x_e) % Q;
                 {
                     LemmaSmallMod(Q- x_e, Q);
@@ -875,10 +661,9 @@ module mulntt_ct_rec {
                 Q - x_e;
             }
   
-
             calc == {
                 diff;
-                modsub(e, modmul(o, x_e));
+                mqsub(e, mqmul(o, x_e));
                 {
                     LemmaMulNonnegative(o, x_e);
                 }
@@ -909,9 +694,9 @@ module mulntt_ct_rec {
                     LemmaSmallMod(e, Q);
                 }
                 (e + (x_o * o) % Q) % Q;
-                (e + modmul(x_o, o)) % Q;
-                modadd(e, modmul(x_o, o));
-                modadd(poly_eval(e_poly, sqr), modmul(x_o, poly_eval(o_poly, sqr)));
+                (e + mqmul(x_o, o)) % Q;
+                mqadd(e, mqmul(x_o, o));
+                mqadd(poly_eval(e_poly, sqr), mqmul(x_o, poly_eval(o_poly, sqr)));
                 {
                     poly_eval_split_lemma(f_poly, e_poly, o_poly, hsize, x_o);
                 }
@@ -924,14 +709,14 @@ module mulntt_ct_rec {
             requires bi < hcount.full
         {
             var s := bi + (2*j) * hcount.full;
-            var w := modmul(x_value(2 * j, hcount), R);
+            var w := mqmul(x_value(2 * j, hcount), R);
             point_view_index_bound_lemma(bi, 2 * j+1, hsize);
             point_view_index_bound_lemma(bi, 2 * j, hsize);
             LemmaMulIsDistributive(hcount.full, 2*j, 1);
             assert (2*j) * hcount.full + hcount.full == (2*j + 1) * hcount.full;
             var s' := s+hcount.full; 
-            a' == a[s := modadd(a[s], montmul(a[s'], w))]
-                [s' := modsub(a[s], montmul(a[s'], w))]
+            a' == a[s := mqadd(a[s], montmul(a[s'], w))]
+                [s' := mqsub(a[s], montmul(a[s'], w))]
         }
 
         lemma s_loop_perserves_higher_inv_lemma(a: n_sized, a': n_sized, hcount: pow2_t, j: nat, bi: nat)
@@ -947,8 +732,8 @@ module mulntt_ct_rec {
             assert s == point_view_index(bi, 2*j, hsize);
             assert s' == point_view_index(bi, 2*j + 1, hsize);
 
-            // var vo := modadd(a[s], modmul(a[s'], w));
-            // var ve := modsub(a[s], modmul(a[s'], w));
+            // var vo := mqadd(a[s], mqmul(a[s'], w));
+            // var ve := mqsub(a[s], mqmul(a[s'], w));
 
             var hpoints := level_points_view(a, hsize);
             var hpoints' := level_points_view(a', hsize);
@@ -956,8 +741,8 @@ module mulntt_ct_rec {
 
             forall i | (0 <= i < bi || bi + 1 <= i < hcount.full)
                 ensures hpoints[i] == hpoints'[i];
-                ensures 0 <= i < bi ==> points_eval_prefix_inv(hpoints'[i], higher[bit_rev_int(i, hcount)], 2*j+2, hcount);
-                ensures bi + 1 <= i < hcount.full ==> points_eval_prefix_inv(hpoints'[i], higher[bit_rev_int(i, hcount)], 2*j, hcount);
+                ensures 0 <= i < bi ==> points_eval_prefix_inv(hpoints'[i], higher[bit_rev_int(i, hcount)], x_value, 2*j+2, hcount);
+                ensures bi + 1 <= i < hcount.full ==> points_eval_prefix_inv(hpoints'[i], higher[bit_rev_int(i, hcount)], x_value, 2*j, hcount);
             {
                 var left := hpoints[i];
                 var right := hpoints'[i];
@@ -977,7 +762,7 @@ module mulntt_ct_rec {
             var right := hpoints'[bi];
             var poly := higher[bit_rev_int(bi, hcount)];
 
-            assert points_eval_prefix_inv(right, poly, 2*j+2, hcount) by {
+            assert points_eval_prefix_inv(right, poly, x_value, 2*j+2, hcount) by {
                 reveal points_eval_prefix_inv();
                 forall k | 0 <= k < 2*j+2 
                     ensures poly_eval(poly, x_value(k, hcount)) == right[k];
@@ -987,7 +772,7 @@ module mulntt_ct_rec {
                         point_view_index_disjont_lemma(bi, k, bi, 2*j+1, hsize);
                         assert right[k] == left[k];
                     } else {
-                        var w := modmul(x_value(2 * j, hcount), R);
+                        var w := mqmul(x_value(2 * j, hcount), R);
                         ct_butterfly_even_lemma(a, hcount, j, bi, s, w);
                         ct_butterfly_odd_lemma(a, hcount, j, bi, s, w);
                     }
@@ -1015,7 +800,7 @@ module mulntt_ct_rec {
             var count := lcount();
 
             forall i | (bi + 1 <= i < hcount.full || bi + hcount.full + 1 <= i < count.full) 
-                ensures points_eval_suffix_inv(lpoints'[i], lower[bit_rev_int(i, count)], j, count);
+                ensures points_eval_suffix_inv(lpoints'[i], lower[bit_rev_int(i, count)], x_value, j, count);
             {
                 var left := lpoints[i];
                 var right := lpoints'[i];
@@ -1032,14 +817,14 @@ module mulntt_ct_rec {
             }
         
             forall i | (0 <= i <= bi || hcount.full <= i <= bi + hcount.full)
-                ensures points_eval_suffix_inv(lpoints'[i], lower[bit_rev_int(i, count)], j+1, count);
+                ensures points_eval_suffix_inv(lpoints'[i], lower[bit_rev_int(i, count)], x_value, j+1, count);
             {
                 var left := lpoints[i];
                 var right := lpoints'[i];
                 var poly := lower[bit_rev_int(i, count)];
 
                 if i == bi || i == bi + hcount.full {
-                    assert points_eval_suffix_inv(right, poly, j+1, count) by {
+                    assert points_eval_suffix_inv(right, poly, x_value, j+1, count) by {
                         reveal points_eval_suffix_inv();
                         forall k | j + 1 <= k < lsize.full
                             ensures right[k] == left[k];
@@ -1100,7 +885,7 @@ module mulntt_ct_rec {
                 var lpoints := level_points_view(a, lsize());
 
                 forall i | (0 <= i < hcount.full || hcount.full <= i < lcount.full)
-                    ensures points_eval_suffix_inv(lpoints[i], lower[bit_rev_int(i, lcount)], j, lcount);
+                    ensures points_eval_suffix_inv(lpoints[i], lower[bit_rev_int(i, lcount)], x_value, j, lcount);
                 {
                     assert (0 <= i < hcount.full || hcount.full <= i < lcount.full)
                         ==> (0 <= i < lcount.full);
@@ -1117,7 +902,7 @@ module mulntt_ct_rec {
                 var hpoints := level_points_view(a, hsize);
                 reveal s_loop_higher_inv();
                 forall i | 0 <= i < |hpoints|
-                    ensures points_eval_prefix_inv(hpoints[i], higher[bit_rev_int(i, hcount)], 2*j+2, hcount);
+                    ensures points_eval_prefix_inv(hpoints[i], higher[bit_rev_int(i, hcount)], x_value, 2*j+2, hcount);
                 {
                 }
                 reveal j_loop_higher_inv();
@@ -1130,7 +915,7 @@ module mulntt_ct_rec {
                 var lpoints := level_points_view(a, lsize());
                 reveal s_loop_lower_inv();
                 forall i | 0 <= i < |lpoints|
-                    ensures points_eval_suffix_inv(lpoints[i], lower[bit_rev_int(i, lcount)], j+1, lcount);
+                    ensures points_eval_suffix_inv(lpoints[i], lower[bit_rev_int(i, lcount)], x_value, j+1, lcount);
                 {
                 }
                 reveal j_loop_lower_inv();
@@ -1144,11 +929,11 @@ module mulntt_ct_rec {
             assert j_loop_higher_inv(a, hcount, 0) by {
                 var hpoints := level_points_view(a, hsize);
                 forall i | 0 <= i < hcount.full
-                    ensures points_eval_prefix_inv(hpoints[i], higher[bit_rev_int(i, hcount)], 0, hcount);
+                    ensures points_eval_prefix_inv(hpoints[i], higher[bit_rev_int(i, hcount)], x_value, 0, hcount);
                 {
                     unifromly_sized_instance_lemma(hpoints, hsize, i);
                     unifromly_sized_instance_lemma(higher, hsize, bit_rev_int(i, hcount));
-                    points_eval_prefix_inv_vacuous_lemma(hpoints[i], higher[bit_rev_int(i, hcount)], hcount);
+                    points_eval_prefix_inv_vacuous_lemma(hpoints[i], higher[bit_rev_int(i, hcount)], x_value, hcount);
                 }
                 reveal j_loop_higher_inv();
             }
@@ -1158,7 +943,7 @@ module mulntt_ct_rec {
                 var lcount := lcount();
                 var lpoints := level_points_view(a, lsize());
                 forall i | 0 <= i < lcount.full
-                    ensures points_eval_suffix_inv(lpoints[i], lower[bit_rev_int(i, lcount)], 0, lcount)
+                    ensures points_eval_suffix_inv(lpoints[i], lower[bit_rev_int(i, lcount)], x_value, 0, lcount)
                 {
                     reveal points_eval_suffix_inv();
                 }
@@ -1168,12 +953,12 @@ module mulntt_ct_rec {
 
         function next_t_loop_view(hcount: pow2_t): (v': loop_view)
             requires loop_view_wf();
-            requires 0 <= hsize.exp <= LOGN;
-            requires 0 <= hcount.exp < LOGN;
+            requires 0 <= hsize.exp <= N.exp;
+            requires 0 <= hcount.exp < N.exp;
             requires hsize == block_size(hcount);
             ensures v'.loop_view_wf();
         {
-            if hsize.exp == LOGN then
+            if hsize.exp == N.exp then
                 this
             else
                 var v' := loop_view(higher, build_higher_level(higher, hsize), pow2_double(hsize));
@@ -1185,17 +970,17 @@ module mulntt_ct_rec {
             returns (v': loop_view)
             requires j_loop_inv(a, hcount, j);
             requires j == lsize().full;
-            requires 0 <= hsize.exp <= LOGN;
+            requires 0 <= hsize.exp <= N.exp;
             ensures v' == next_t_loop_view(hcount);
-            ensures hsize.exp < LOGN ==> v'.t_loop_inv(a, pow2_half(hcount));
-            ensures hsize.exp == LOGN ==> v'.t_loop_end(a);
+            ensures hsize.exp < N.exp ==> v'.t_loop_inv(a, pow2_half(hcount));
+            ensures hsize.exp == N.exp ==> v'.t_loop_end(a);
         {
             reveal j_loop_higher_inv();
             size_count_lemma();
             var hpoints := level_points_view(a, hsize);
 
             forall i | 0 <= i < hcount.full
-                ensures points_eval_inv(hpoints[i], higher[bit_rev_int(i, hcount)], hcount);
+                ensures points_eval_inv(hpoints[i], higher[bit_rev_int(i, hcount)], x_value, hcount);
             {
                 reveal points_eval_suffix_inv();
                 reveal points_eval_prefix_inv();
@@ -1204,16 +989,17 @@ module mulntt_ct_rec {
             v' := next_t_loop_view(hcount);
             v'.size_count_lemma();
 
-            if hsize.exp < LOGN {
+            if hsize.exp < N.exp {
                 assert v'.t_loop_inv(a, pow2_half(hcount)) by {
                     reveal v'.t_loop_low_inv();
                     assert v'.t_loop_low_inv(a, v'.hcount());
                 }
             } else {
                 Nth_root_lemma();
-                assert hsize.exp == LOGN;
-                assert hsize.full == N;
-                assert |hpoints| * N == N;
+                assert hsize.exp == N.exp;
+                assert hsize.full == N.full;
+                assert |hpoints| * N.full == N.full;
+                LemmaFundamentalDivModConverse(|hpoints| * N.full, N.full, 1, 0);
                 assert |hpoints| == 1;
                 assert bit_rev_int(0, hcount) == 0;
             }
